Splinter/AllocationsLayer/CoordinationSystemRefinement.i.dfy
@@ -6,18 +6,21 @@ include "FullStackBetreeRefinement.i.dfy"
 include "FullStackJournalRefinement.i.dfy"
 
 module CoordinationSystemRefinement {
+  import opened ValueMessage
+  import opened MsgHistoryMod
   import opened GenericDisk
+  import opened CoordinationSystemMod
   import FullStackJournalRefinement
   import FullStackBetreeRefinement
-  import opened CoordinationSystemMod
-  import AllocationBetreeMod
+  import AllocationJournalRefinement
+
+  // import AllocationBetreeMod
   // import AbstractSystem = CoordinationSystem
 //   import opened Options
 //   import opened MapRemove_s
 //   import opened CrashTolerantMapSpecMod
 //   import opened MsgHistoryMod
 //   import opened KeyType
-//   import opened ValueMessage
 //   import opened TotalKMMapMod
 //   import opened LSNMod
 //   import opened CoordinationJournal
@@ -46,6 +49,7 @@ module CoordinationSystemRefinement {
 
   predicate DisjointEphemeralComponents(v: Variables)
   {
+    // chained disjoint means all pairs are disjoint
     && (KnownEphemeral(v) ==> v.freeset.ephemeral !! v.betree.EphemeralAUs() !! v.journal.EphemeralAUs())
   }
 
@@ -71,18 +75,23 @@ module CoordinationSystemRefinement {
     v.freeset.persistent + v.betree.PersistentAUs() + v.journal.PersistentAUs()
   }
 
-  function TotalInflight(v: Variables) : set<AU>
-    requires InFlightBetreeOnly(v) || InFlightAllReady(v)
+  function TotalInflightBetreeOnly(v: Variables) : set<AU>
+    requires InFlightBetreeOnly(v)
   {
-    if InFlightAllReady(v)
-    then v.freeset.inFlight.value + v.betree.InFlightAUs() + v.journal.InFlightAUs()
-    else v.freeset.inFlight.value + v.betree.InFlightAUs() + v.journal.EphemeralAUs()
+    v.freeset.inFlight.value + v.betree.InFlightAUs() + v.journal.EphemeralAUs()
+  }
+
+  function TotalInflight(v: Variables) : set<AU>
+    requires InFlightAllReady(v)
+  {
+    v.freeset.inFlight.value + v.betree.InFlightAUs() + v.journal.InFlightAUs()
   }
 
   predicate StatesPreservesTotalAUs(v: Variables)
   {
     && (KnownEphemeral(v) ==> TotalEphemeral(v) == TotalPersistent(v))
-    && (InFlightBetreeOnly(v) || InFlightAllReady(v) ==> TotalInflight(v) == TotalPersistent(v))
+    && (InFlightBetreeOnly(v) ==> TotalInflightBetreeOnly(v) == TotalPersistent(v))
+    && (InFlightAllReady(v) ==> TotalInflight(v) == TotalPersistent(v))
   }
 
   predicate Inv(v: Variables)
@@ -97,7 +106,7 @@ module CoordinationSystemRefinement {
     && DisjointEphemeralComponents(v)
     && DisjointInFlightComponents(v)
     && DisjointPersistentComponents(v)
-    && StatesPreservesTotalAUs(v)
+    && StatesPreservesTotalAUs(v) // not necessary for pure safety 
   }
 
   function I(v: Variables) : AbstractSystem.Variables
@@ -106,7 +115,7 @@ module CoordinationSystemRefinement {
     var journal := FullStackJournalRefinement.I(v.journal);
     var mapadt := FullStackBetreeRefinement.I(v.betree);
     AbstractSystem.Variables(journal, mapadt, v.ephemeral)
-  } 
+  }
 
   lemma InitRefines(v: Variables, availAUs: set<AU>)
     requires Init(v, availAUs)
@@ -116,6 +125,197 @@ module CoordinationSystemRefinement {
     FullStackBetreeRefinement.InitRefines(v.betree);
   }
 
+  lemma LoadEphemeralFromPersistentRefines(v: Variables, v': Variables, uiop: UIOp)
+    requires Inv(v)
+    requires LoadEphemeralFromPersistent(v, v', uiop)
+    ensures Inv(v')
+    ensures AbstractSystem.Next(I(v), I(v'), uiop)
+  {
+    var journalLbl := CoordinationJournal.LoadEphemeralFromPersistentLabel();
+    var betreeLbl := CoordinationBetree.LoadEphemeralFromPersistentLabel(v'.ephemeral.mapLsn);
+    
+    FullStackJournalRefinement.NextRefines(v.journal, v'.journal, journalLbl);
+    FullStackBetreeRefinement.NextRefines(v.betree, v'.betree, betreeLbl);
+
+    assert v'.journal.persistent == v.journal.persistent;
+    assert v'.betree.persistent == v.betree.persistent;
+    assert v'.journal.EphemeralAUs() == v.journal.PersistentAUs() by {
+      AllocationJournalRefinement.reveal_LikesJournalInv();
+    }
+    assume v'.betree.EphemeralAUs() == v.betree.PersistentAUs(); // maintained by betree Inv
+
+    assert DisjointEphemeralComponents(v');
+    assert StatesPreservesTotalAUs(v');
+
+    assert AbstractSystem.NextStep(I(v), I(v'), uiop, AbstractSystem.LoadEphemeralFromPersistentStep());
+  }
+
+  lemma RecoverRefines(v: Variables, v': Variables, uiop: UIOp, step: Step)
+    requires Inv(v)
+    requires step.RecoverStep?
+    requires NextStep(v, v', uiop, step)
+    ensures Inv(v')
+    ensures AbstractSystem.Next(I(v), I(v'), uiop)
+  {
+    var journalLbl := CoordinationJournal.ReadForRecoveryLabel(step.records);
+    var betreeLbl := CoordinationBetree.PutRecordsLabel(step.records);
+    
+    FullStackJournalRefinement.NextRefines(v.journal, v'.journal, journalLbl);
+    FullStackBetreeRefinement.NextRefines(v.betree, v'.betree, betreeLbl);
+
+    CoordinationBetree.EphemeralAUsSameAfterPut(v.betree, v'.betree, betreeLbl);
+    assert v'.betree.EphemeralAUs() == v.betree.EphemeralAUs();
+    assert v'.journal.EphemeralAUs() == v.journal.EphemeralAUs();
+
+    assert AbstractSystem.NextStep(I(v), I(v'), uiop, AbstractSystem.RecoverStep(step.records));
+  }
+
+  lemma QueryRefines(v: Variables, v': Variables, uiop: UIOp, step: Step)
+    requires Inv(v)
+    requires step.QueryStep?
+    requires NextStep(v, v', uiop, step)
+    ensures Inv(v')
+    ensures AbstractSystem.Next(I(v), I(v'), uiop)
+  {
+    var key := uiop.baseOp.req.input.key;
+    var value := uiop.baseOp.reply.output.value;
+    var journalLbl := CoordinationJournal.QueryEndLsnLabel(v.ephemeral.mapLsn);
+    var betreeLbl := CoordinationBetree.QueryLabel(v.ephemeral.mapLsn, key, value);
+    
+    FullStackJournalRefinement.NextRefines(v.journal, v'.journal, journalLbl);
+    FullStackBetreeRefinement.NextRefines(v.betree, v'.betree, betreeLbl);
+
+    assert AbstractSystem.NextStep(I(v), I(v'), uiop, AbstractSystem.QueryStep());
+  }
+
+  lemma PutRefines(v: Variables, v': Variables, uiop: UIOp, step: Step)
+    requires Inv(v)
+    requires step.PutStep?
+    requires NextStep(v, v', uiop, step)
+    ensures Inv(v')
+    ensures AbstractSystem.Next(I(v), I(v'), uiop)
+  {
+    var key := uiop.baseOp.req.input.key;
+    var val := uiop.baseOp.req.input.value;
+    var singleton := MsgHistoryMod.SingletonAt(v.ephemeral.mapLsn, KeyedMessage(key, Define(val)));
+    var journalLbl := CoordinationJournal.PutLabel(singleton);
+    var betreeLbl := CoordinationBetree.PutRecordsLabel(singleton);
+
+    FullStackJournalRefinement.NextRefines(v.journal, v'.journal, journalLbl);
+    FullStackBetreeRefinement.NextRefines(v.betree, v'.betree, betreeLbl);
+    CoordinationBetree.EphemeralAUsSameAfterPut(v.betree, v'.betree, betreeLbl);
+    assert v'.betree.EphemeralAUs() == v.betree.EphemeralAUs();
+    assert v'.journal.EphemeralAUs() == v.journal.EphemeralAUs();
+    
+    assert AbstractSystem.NextStep(I(v), I(v'), uiop, AbstractSystem.PutStep());
+  }
+
+  lemma ReqSyncRefines(v: Variables, v': Variables, uiop: UIOp, step: Step)
+    requires Inv(v)
+    requires step.ReqSyncStep?
+    requires NextStep(v, v', uiop, step)
+    ensures Inv(v')
+    ensures AbstractSystem.Next(I(v), I(v'), uiop)
+  {
+    var journalLbl := CoordinationJournal.QueryEndLsnLabel(v.ephemeral.mapLsn);
+    FullStackJournalRefinement.NextRefines(v.journal, v'.journal, journalLbl);
+    assert v'.journal.EphemeralAUs() == v.journal.EphemeralAUs();
+    assert AbstractSystem.NextStep(I(v), I(v'), uiop, AbstractSystem.ReqSyncStep());
+  }
+
+  lemma ReplySyncRefines(v: Variables, v': Variables, uiop: UIOp, step: Step)
+    requires Inv(v)
+    requires step.ReplySyncStep?
+    requires NextStep(v, v', uiop, step)
+    ensures Inv(v')
+    ensures AbstractSystem.Next(I(v), I(v'), uiop)
+  {
+    var journalLbl := CoordinationJournal.QueryLsnPersistenceLabel(v.ephemeral.syncReqs[uiop.syncReqId]);
+    FullStackJournalRefinement.NextRefines(v.journal, v'.journal, journalLbl);
+    assert v'.journal.EphemeralAUs() == v.journal.EphemeralAUs();
+    assert AbstractSystem.NextStep(I(v), I(v'), uiop, AbstractSystem.ReplySyncStep());
+  }
+
+  lemma CrashRefines(v: Variables, v': Variables, uiop: UIOp, step: Step)
+    requires Inv(v)
+    requires step.CrashStep?
+    requires NextStep(v, v', uiop, step)
+    ensures Inv(v')
+    ensures AbstractSystem.Next(I(v), I(v'), uiop)
+  {
+    var journalLbl := CoordinationJournal.CrashLabel();
+    var betreeLbl := CoordinationBetree.CrashLabel();
+
+    FullStackJournalRefinement.NextRefines(v.journal, v'.journal, journalLbl);
+    FullStackBetreeRefinement.NextRefines(v.betree, v'.betree, betreeLbl);
+    assert AbstractSystem.NextStep(I(v), I(v'), uiop, AbstractSystem.CrashStep());
+  }
+
+  lemma JournalInternalRefines(v: Variables, v': Variables, uiop: UIOp, step: Step)
+    requires Inv(v)
+    requires step.JournalInternalStep?
+    requires NextStep(v, v', uiop, step)
+    ensures Inv(v')
+    ensures AbstractSystem.Next(I(v), I(v'), uiop)
+  {
+    assert v'.journal.inFlight == v.journal.inFlight;
+    assert v'.journal.persistent == v.journal.persistent;
+
+    var journalLbl := CoordinationJournal.InternalLabel(step.allocs, step.deallocs);
+    assert FullStackJournalRefinement.FreshLabel(v.journal, journalLbl);
+
+    FullStackJournalRefinement.NextRefines(v.journal, v'.journal, journalLbl);
+    FullStackJournalRefinement.InternalLabelAccessibleAUs(v.journal, v'.journal, journalLbl);
+
+    assert v.journal.EphemeralAUs() + step.allocs - step.deallocs == v'.journal.EphemeralAUs();
+
+    if InFlightBetreeOnly(v) {
+      assert InFlightBetreeOnly(v'); 
+
+      /*
+      predicate DisjointInFlightComponents(v: Variables) {
+        && (InFlightBetreeOnly(v) ==> v.freeset.inFlight.value !! v.betree.InFlightAUs() !! v.journal.EphemeralAUs())
+      }
+        
+      predicate preserves total AUs
+        && (InFlightBetreeOnly(v) ==> TotalInflightBetreeOnly(v) == TotalPersistent(v)
+
+      TotalInflightBetreeOnly(v) == v.freeset.inFlight.value + v.betree.InFlightAUs() + v.journal.EphemeralAUs()
+      
+      */
+          // assert step.allocs !! v'.betree.EphemeralAUs();
+    // assert step.allocs !! v'.freeset.ephemeral;
+    // assert step.allocs !! v.journal.EphemeralAUs();
+    
+    }
+
+    //   && (InFlightBetreeOnly(v) ==> TotalInflightBetreeOnly(v) == TotalPersistent(v))
+    // && ((v) ==> TotalInflight(v) == TotalPersistent(v))
+
+    // if InFlightBetreeOnly(v) {
+    //   assert InFlightBetreeOnly(v');
+    //   assert TotalInflight(v) == TotalPersistent(v);
+    //   assert TotalInflight(v') == TotalPersistent(v');
+
+  //   function TotalInflight(v: Variables) : set<AU>
+  //   requires InFlightBetreeOnly(v) || InFlightAllReady(v)
+  // {
+  //   if InFlightAllReady(v)
+  //   then v.freeset.inFlight.value + v.betree.InFlightAUs() + v.journal.InFlightAUs()
+  //   else v.freeset.inFlight.value + v.betree.InFlightAUs() + v.journal.EphemeralAUs()
+  // }
+
+    // }
+
+    // assert StatesPreservesTotalAUs(v');
+
+    assume false;
+    assert DisjointEphemeralComponents(v');
+    assert AbstractSystem.NextStep(I(v), I(v'), uiop, AbstractSystem.JournalInternalStep());
+
+  }
+
+
   lemma NextRefines(v: Variables, v': Variables, uiop: UIOp)
     requires Inv(v)
     requires Next(v, v', uiop)
@@ -124,24 +324,21 @@ module CoordinationSystemRefinement {
   {
     var step :| NextStep(v, v', uiop, step);
     match step {
-      // case LoadEphemeralFromPersistentStep() => LoadEphemeralFromPersistent(v, v', uiop)
-      // case RecoverStep(records) => Recover(v, v', uiop, records)
-      // case AcceptRequestStep() => AcceptRequest(v, v', uiop)
-      // case QueryStep() => Query(v, v', uiop)
-      // case PutStep() => Put(v, v', uiop)
-      // case DeliverReplyStep() => DeliverReply(v, v', uiop)
+      case LoadEphemeralFromPersistentStep() => LoadEphemeralFromPersistentRefines(v, v', uiop);
+      case RecoverStep(records) => RecoverRefines(v, v', uiop, step);
+      case AcceptRequestStep() => assert AbstractSystem.NextStep(I(v), I(v'), uiop, AbstractSystem.AcceptRequestStep());
+      case QueryStep() => QueryRefines(v, v', uiop, step);
+      case PutStep() => PutRefines(v, v', uiop, step);
+      case DeliverReplyStep() => assert AbstractSystem.NextStep(I(v), I(v'), uiop, AbstractSystem.DeliverReplyStep());
       // case JournalInternalStep(allocs, deallocs) => JournalInternal(v, v', uiop, allocs, deallocs)
       // case MapInternalStep(allocs, deallocs) => MapInternal(v, v', uiop, allocs, deallocs)
-      // case ReqSyncStep() => ReqSync(v, v', uiop)
-      // case ReplySyncStep() => ReplySync(v, v', uiop)
+      case ReqSyncStep() => ReqSyncRefines(v, v', uiop, step);
+      case ReplySyncStep() => ReplySyncRefines(v, v', uiop, step);
       // case FreezeBetreeStep(unobservedBetree, unobservedJournal) => FreezeBetree(v, v', uiop, unobservedBetree, unobservedJournal)
       // case CommitStartStep(newBoundaryLsn) => CommitStart(v, v', uiop, newBoundaryLsn)
       // case CommitCompleteStep(discardedJournal) => CommitComplete(v, v', uiop, discardedJournal)
-      // case CrashStep() => Crash(v, v', uiop)
+      case CrashStep() => CrashRefines(v, v', uiop, step);
       case _ => assume false;
     }
-    // requires lbl.InternalLabel? ==> AllocationBetreeRefinement.FreshLabel(v.ephemeral.v, AllocLbl(v, v', lbl))
-    // FullStackBetreeRefinement.NextRefines(v.betree, v'.betree);
-    // FullStackJournalRefinement.NextRefines(v.journal, v'.journal);
   }
 }
